---
layout: home_page 
sidebar: false
title: Solutions to Rudin's Principles of Mathematical Analysis
author: Daniel McNeela
description: Exercises from Chapter 1 of the book.
excerpt_separator: <!--more-->
categories: math
preview_img: images/rudin.jpg
---

**Exercise 1:** *If $$r$$ is rational ($$r \neq 0$$) and $$x$$ is irrational,
prove that $$r + x$$ and $$rx$$ are irrational.*

Suppose $$r \in \mathbb{Q}$$ and $$x \in \mathbb{I}$$ but $$r+x,\ rx \in \mathbb{Q}$$.
Then we have $$r +x = \frac{a}{b}$$ for some $$a,b \in \mathbb{Z}$$. This
implies that $$x = \frac{a}{b} - r$$. Since $$r \in \mathbb{Q}$$, $$r = \frac{c}{d}$$
for some $$c, d \in \mathbb{Z}$$. Therefore
	\\[x = \frac{a}{b} - \frac{c}{d} = \frac{ad-bc}{bd}\\]
which implies $$x \in \mathbb{Q}$$: a contradiction. Therefore, $$r + x$$ is irrational.
Now, consider $$rx$$. If $$rx \in \mathbb{Q}$$, then

\begin{align}
	rx &= \frac{a}{b}\ \text{for}\ a,b \in \mathbb{Z} \\
	\implies x &= \frac{a}{b} \cdot \frac{d}{c} \\
	\implies x &\in \mathbb{Q}
\end{align}

which is a contradiction. Therefore, $$rx$$ is irrational.
<!--more-->
\\
\\
**Exercise 2:** *Prove that there is no rational whose square is $$12$$.*
\\
\\
Suppose there exists a rational $$p$$ such that $$p^2 = 12$$.
Since $$p \in \mathbb{Q}$$, we can write $$p = \frac{m}{n}$$ where the
fraction $$\frac{m}{n}$$ is in lowest terms, i.e. $$m$$ and $$n$$ are
not both even. Then we have
	\\[\frac{m^2}{n^2} = 12 \implies m^2=4\cdot 3n^2 \implies \frac{m^2}{4} = 3n^2\\]
Since $$3n^2$$ is an integer, $$\frac{m^2}{4}$$ must be divisible by $$4$$ and hence even.
Since only one of $$m$$ and $$n$$ can be even, this implies that $$n$$ is odd, from which
it follows that $$3n^2$$ is odd. But if $$3n^2$$ is odd and $$\frac{m^2}{4}$$ is even then
we must have
	\\[\frac{m^2}{4} \neq 3n^2\\]
Therefore, there is no rational whose square is $$12$$.
\\
\\
Prove Proposition 1.15.
(a) We have
\begin{align}
	y = 1\cdot y = \left(\frac{1}{x} \cdot x\right) \cdot y = \frac{1}{x} \cdot (xy) =
	\frac{1}{x} \cdot(xz) = \left(\frac{1}{x} \cdot x \right) \cdot z = 1 \cdot z = z
\end{align}
(b) If $$xy = x$$ then $$xy = x \cdot 1$$, so by (a) we have $$y=1$$.
\\
(c) If $$xy = 1$$ then
\begin{align}
	y = 1 \cdot y = \left(\frac{1}{x} \cdot x \right) \cdot y
	= \frac{1}{x} \cdot (xy) = \frac{1}{x} \cdot 1 = \frac{1}{x}
\end{align}
(d) We have
\begin{align}
	\dfrac{1}{(1/x)} = 1 \cdot \dfrac{1}{(1/x)} = \left( \frac{1}{x} \cdot x \right) \cdot
	\dfrac{1}{(1/x)} = \left(\frac{1}{x} \cdot \dfrac{1}{(1/x)} \right) \cdot x = 1 \cdot x = x
\end{align}
Let $$E$$ be a nonempty subset of an ordered set; suppose $$\alpha$$ is a lower bound
of $$E$$ and $$\beta$$ is an upper bound of $$E$$. Prove that $$\alpha \leq \beta$$.
\ Because $$E$$ is nonempty, there exists $$x \in E$$. Since $$\alpha$$ is a lower bound of $$E$$, we 
have $$\alpha \leq x$$. Since $$\beta$$ is an upper bound of $$E$$, we have $$x \leq \beta$$. Therefore
	\\[\alpha \leq x \leq \beta \implies \alpha \leq \beta\\]
	Let $$A$$ be a nonempty set of real numbers which is bounded below. Let $$-A$$ be the
set of all numbers $$-x$$, where $$x \in A$$. Prove that
	$$\inf A = - \sup(-A)$$
	Let $$\alpha = \sup(-A)$$. Then for each $$x \in -A$$ we have $$x \leq \alpha$$. Therefore, we have
$$-x \geq -\alpha$$ for each $$-x \in A$$, so $$-\alpha$$ is a lower bound for $$A$$.
Now, suppose there exists a lower bound $$\beta$$ of $$A$$ such that $$\beta > -\alpha$$. Then
\begin{align}
	-x \geq \beta > \alpha \quad \forall -x \in A \implies x \leq -\beta < \alpha \quad \forall x \in -A
	\implies \alpha \neq \sup(-A)
\end{align}
which is a contradiction. Therefore, $$-\alpha = \inf A$$ which implies that
	\\[\inf A = -\sup (-A)\\]
(a) We have
\begin{align}
	(b^m)^{1/n} = (b^m)^{r/m} =b^r = b^{p/q} = (b^p)^{1/q} 
\end{align}
(b) We have
\begin{align}
	b^{r+s} = b^{\frac{m}{n} + \frac{p}{q}} = b^{\frac{mq + np}{nq}}
	= (b^{mq}b^{np})^{\frac{1}{nq}} = b^{\frac{m}{n}}b^{\frac{p}{q}} = b^rb^s
\end{align}
(c) Let $$b^t \in B(r)$$. We have
\begin{align}
	b^t \cdot b^{r-t} = b^r
\end{align}
Since $$r \geq t$$ for every $$t$$, we know that $$b^{r-t} \geq 1 \implies b^r \geq b^t$$.
Therefore $$b^r$$ is an upper bound for $$B(r)$$.

Now, suppose $$c$$ is an upper bound for $$B(r)$$ and $$c < b^r$$. Then
$$c = b^{r - \varepsilon}$$ for some $$\varepsilon \in \mathbb{Q}$$. Since $$\mathbb{Q}$$ is dense in $$\mathbb{R}$$,
there exists $$t$$ such that $$r - \varepsilon < t < r$$. Therefore $$b^t > c$$
and $$b^t \in B(r)$$ so $$c$$ is not an upper bound for $$B(r)$$, a contradiction.
Therefore, $$b^r = \sup B(r)$$. \
(d) We have
\begin{align}
	b^{x+y} = \sup B(x+y)
\end{align}
where $$x \in B(x)$$ and

**Exercise** Fix $$b > 1$$, $$y > 0$$, and prove that there is a unique real $$x$$
such that $$b^x = y$$, by completing the following outline. (This $$x$$ is
called the \textit{logarithm of y to the base b}.) \\
(a) For any positive integer $$n$$, $$b^n - 1 \geq n(b-1)$$. \\
(b) Hence $$b - 1 \geq n(b^{1/n}-1)$$. \\
(c) If $$t > 1$$ and $$n > (b-1)/(t-1)$$, then $$b^{1/n} < t$$. \\
(d) If $$w$$ is such that $$b^w < y$$, then $$b^{w + (1/n)}y < y$$ for sufficiently large $$n$$. \\
(e) If $$b^2 > y$$, then $$b^{w - (1/n)} > y$$ for sufficiently large $$n$$. \\
(f) Let $$A$$ be the set of all $$w$$ such that $$b^w < y$$, and show that $$x = \sup A$$ satisfies $$b^x = y$$. \\
(g) Prove that this $$x$$ is unique.


(a) Note that

\begin{align}
	b^n-1 &= b^{n-1}\cdot b-1 \\
			&= (b-1)b^{n-1} + b^{n-1} - 1 \
			&= (b-1)b^{n-1} + (b-1)b^{n-2} + b^{n-2} - 1 \
			&\ \ \vdots \\
			& = (b-1)(b^{n-1} + b^{n-2} + \cdots + b + 1)
\end{align}

Since each of $$b^{n-1}, b^{n-2}, \dots, b, 1 \geq 1$$ we have

\begin{align}
	(b-1)(b^{n-1} + b^{n-2} + \cdots + b + 1) \geq (b-1)\underbrace{(1 + 1 + \cdots + 1)}_{n\text{-times}} = n(b-1)
\end{align}

(b) Fix $$n$$ and set $$b = a^{1/n}$$. Then by part (a) we have

\begin{align}
	b^n -1 \geq n(b-1) \implies (a^{1/n})^n - 1 \geq n(a^{1/n} - 1)
	\implies a-1 \geq n(a^{1/n} -1)
\end{align}

(c) Since $$\dfrac{b-1}{t-1} \geq n$$ we have

\begin{align}
	\frac{b-1}{t-1}(b^{1/n}-1) < n(b^{1/n}-1) \leq  b-1 \\
	\implies \frac{1}{t-1}(b^{1/n}-1) < 1 \\
	\implies t - 1 > b^{1/n} - 1 \\
	\implies t > b^{1/n}
\end{align}

